-

Misc.v
@@ -1667,6 +1667,164 @@ Qed.
 
 (* end map2 *)
 
+(* List_find_nth: like find but doesn't return the element found
+   but its rank in the list *)
+
+Fixpoint List_find_nth_loop i A (f : A → bool) (l : list A) :=
+  match l with
+  | [] => None
+  | x :: tl => if f x then Some i else List_find_nth_loop (S i) f tl
+end.
+
+Definition List_find_nth := List_find_nth_loop 0.
+
+Theorem List_find_nth_loop_le : ∀ A f (l : list A) i j,
+  List_find_nth_loop i f l = Some j
+  → i ≤ j.
+Proof.
+intros * Hi.
+revert i j Hi.
+induction l as [| a]; intros; [ easy | ].
+cbn in Hi.
+remember (f a) as b eqn:Hb; symmetry in Hb.
+destruct b. {
+  now injection Hi; clear Hi; intros; subst i.
+}
+specialize (IHl (S i) j Hi).
+flia IHl.
+Qed.
+
+Theorem List_find_nth_loop_Some : ∀ A d f (l : list A) i j,
+  List_find_nth_loop i f l = Some j
+  → f (nth (j - i) l d) = true.
+Proof.
+intros * Hi.
+remember (j - i) as k eqn:Hk.
+replace j with (i + k) in Hi. 2: {
+  specialize (List_find_nth_loop_le f l i Hi) as H1.
+  flia Hk H1.
+}
+clear j Hk.
+revert i l Hi.
+induction k; intros. {
+  rewrite Nat.add_0_r in Hi.
+  revert i Hi.
+  induction l as [| a]; intros; [ easy | ].
+  cbn in Hi |-*.
+  remember (f a) as b eqn:Hb; symmetry in Hb.
+  destruct b; [ easy | exfalso ].
+  specialize (List_find_nth_loop_le f l (S i) Hi) as H1.
+  flia H1.
+}
+destruct l as [| a]; [ easy | ].
+cbn in Hi |-*.
+remember (f a) as b eqn:Hb; symmetry in Hb.
+destruct b. {
+  injection Hi; clear Hi; intros Hi; flia Hi.
+}
+rewrite <- Nat.add_succ_comm in Hi.
+now apply (IHk (S i)).
+Qed.
+
+Theorem List_find_nth_loop_Some' : ∀ A d f (l : list A) i j,
+  List_find_nth_loop i f l = Some j
+  → (∀ k, k < j → f (nth (k - i) l d) = false) ∧
+    f (nth (j - i) l d) = true.
+Proof.
+intros * Hi.
+split; [ | now apply List_find_nth_loop_Some ].
+intros p Hp.
+remember (j - i) as k eqn:Hk.
+replace j with (i + k) in Hi, Hp. 2: {
+  specialize (List_find_nth_loop_le f l i Hi) as H1.
+  flia Hk H1.
+}
+clear j Hk.
+revert i p l Hi Hp.
+induction k; intros. {
+  rewrite Nat.add_0_r in Hi, Hp.
+  revert i Hi Hp.
+  induction l as [| a]; intros; [ easy | ].
+  cbn in Hi |-*.
+  remember (f a) as b eqn:Hb; symmetry in Hb.
+  destruct b. {
+    replace (p - i) with 0 by flia Hp.
+...
+  destruct b; [ easy | exfalso ].
+  specialize (List_find_nth_loop_le f l (S i) Hi) as H1.
+  flia H1.
+}
+destruct l as [| a]; [ easy | ].
+cbn in Hi |-*.
+remember (f a) as b eqn:Hb; symmetry in Hb.
+destruct b. {
+  injection Hi; clear Hi; intros Hi; flia Hi.
+}
+rewrite <- Nat.add_succ_comm in Hi.
+now apply (IHk (S i)).
+Qed.
+
+Theorem List_find_nth_Some : ∀ A d f (l : list A) i,
+  List_find_nth f l = Some i → f (nth i l d) = true.
+Proof.
+intros * Hi.
+unfold List_find_nth in Hi.
+apply List_find_nth_loop_Some with (d := d) in Hi.
+now rewrite Nat.sub_0_r in Hi.
+Qed.
+
+Theorem List_find_nth_Some' : ∀ A d f (l : list A) i,
+  List_find_nth f l = Some i
+  → (∀ j, j < i → f (nth j l d) = false) ∧
+    f (nth i l d) = true.
+Proof.
+intros * Hi.
+unfold List_find_nth in Hi.
+split. 2: {
+  apply List_find_nth_loop_Some with (d := d) in Hi.
+  now rewrite Nat.sub_0_r in Hi.
+}
+intros j Hj.
+...
+Qed.
+
+...
+
+Print find.
+
+Theorem glop : ∀ A d f (l : list A) i,
+  List_find_nth f l = Some i
+  → find f l = Some (nth i l d).
+Proof.
+intros * Hi.
+remember (find f l) as r eqn:Hr.
+symmetry in Hr.
+destruct r as [| j]. {
+  apply find_some in Hr.
+  destruct Hr as (Ha, Hfa).
+  f_equal.
+...
+  apply List_find_nth_Some with (d := d) in Hi.
+...
+intros * Hi.
+(*
+apply List_find_nth_Some with (d := d) in Hi.
+*)
+revert i Hi.
+induction l as [| a]; intros; [ easy | ].
+cbn in Hi.
+cbn - [ nth ].
+remember (f a) as b eqn:Hb; symmetry in Hb.
+destruct b. {
+  now injection Hi; clear Hi; intros; subst i.
+}
+destruct i. {
+  cbn.
+Search find.
+...
+
+(* end List_find_nth *)
+
 (* conversions if ...? into if ..._dec *)
 
 Theorem if_eqb_eq_dec : ∀ A i j (a b : A),
